\documentclass[12pt]{article}
\usepackage[utf8]{inputenc}

\begin{document}
\large

\noindent
$
S\ K\ K \equiv
(\lambda x\ y\ z.x\ z\ (y\ z))\ (\lambda x\ y.x)\ (\lambda x\ y.x) \rightarrow_\beta \\
\rightarrow_\beta (\lambda y\ z.[\lambda x\ y.x]\ z\ (y\ z))\ (\lambda x\ y.x) \rightarrow_\beta \\
\rightarrow_\beta (\lambda y\ z.[\lambda y.z]\ (y\ z))\ (\lambda x\ y.x) \rightarrow_\beta (\lambda y\ z.z)\ (\lambda x\ y.x) \rightarrow_\beta \\
\rightarrow_\beta (\lambda z. z) \equiv I
$

\end{document}